Commit before refactoring atom.subst

src/tactic/nccc/sol.lean
@@ -1,27 +1,40 @@
-import .misc data.list.basic
+import data.list.basic 
 
-variable {α : Type}
+universe u 
 
-def value (α : Type) : Type := list α → (α × Prop)
+variable {α : Type u}
+--def update (m : nat) (a : α) (v : nat → α) : nat → α
+--| n := if n = m then a else v n
+--
+--local notation v `{` m `↦` a `}` := update m a v
 
-def model (α : Type) : Type := nat → value α
+def update_zero (a : α) (f : nat → α) : nat → α
+| 0     := a
+| (k+1) := f k
+
+def denot (α : Type u) : Type u := list α → (α × Prop)
+
+def denot.default [inhabited α] : denot α := 
+λ as, (default α, false)
+
+def model (α : Type u) : Type u := nat → denot α
 
 @[derive has_reflect, derive decidable_eq]
 inductive atom : Type
 | var : nat → atom
 | app : atom → atom → atom
 
-def sub : Type := list (nat × atom)
+local notation `#` := atom.var
+local notation a `&` b := atom.app a b
+
+@[reducible] def sub : Type := list (nat × atom)
 
 def sub.get (σ : sub) (k : nat) : option atom :=
 prod.snd <$> (list.find (eq k ∘ prod.fst)) σ
 
 namespace atom
 
-local notation `#` := atom.var
-local notation a `&` b := atom.app a b
-
-def val (M : model α) : atom → value α
+def val (M : model α) : atom → denot α
 | (# k)   := M k
 | (a & b) := a.val ∘ list.cons (b.val []).fst
 
@@ -41,7 +54,16 @@ lemma subst_eq_of_get_eq_some {σ : sub} {k : nat} {a : atom} :
   σ.get k = some a → (# k).subst σ = a :=
 by {intro h1, simp only [h1, atom.subst]}
 
+def incr_idxs_ge (k : nat) : atom → atom
+| (# m) := if k ≤ m then # (m + 1) else # m
+| (a & b) := incr_idxs_ge a & incr_idxs_ge b 
+
+def incr_idxs : atom → atom := incr_idxs_ge 0
+
 end atom
+
+def sub.incr_idxs : sub → sub :=
+list.map (prod.map nat.succ (atom.incr_idxs))
 
 namespace model
 
@@ -90,6 +112,11 @@ lemma val_subst (M : model α) (σ : sub) :
 
 end atom
 
+def head_occ (k : nat) : atom → Prop
+| (# m)         := k = m 
+| (a & (# m))   := head_occ a
+| (a & (b & c)) := head_occ a ∨ head_occ (b & c)
+
 local notation f `₀↦` a := update_zero a f
 
 @[derive has_reflect]
@@ -102,21 +129,390 @@ inductive form : Type
 | fa  : form → form
 | ex  : form → form
 
-local notation `⊤*`     := form.true
-local notation `⊥*`     := form.false
-local notation `+*`     := form.lit tt
-local notation `-*`     := form.lit ff
-local notation p `∨*` q := form.or p q
-local notation p `∧*` q := form.and p q
-local notation `∀*`     := form.fa
-local notation `∃*`     := form.ex
+local notation `⊤*`            := form.true
+local notation `⊥*`            := form.false
+local notation `⟪` b `,` a `⟫` := form.lit b a
+local notation p `∨*` q        := form.or p q
+local notation p `∧*` q        := form.and p q
+local notation `∀*`            := form.fa
+local notation `∃*`            := form.ex
 
 def holds : model α → form → Prop
 | M ⊤*       := _root_.true
 | M ⊥*       := _root_.false
-| M (+* a)   :=    (a.val M []).snd
-| M (-* a)   :=  ¬ (a.val M []).snd
+| M ⟪tt, a⟫  :=    (a.val M []).snd
+| M ⟪ff, a⟫  :=  ¬ (a.val M []).snd
 | M (p ∨* q) := holds M p ∨ holds M q
 | M (p ∧* q) := holds M p ∧ holds M q
-| M (∀* p)   := ∀ x : value α, holds (M ₀↦ x) p
-| M (∃* p)   := ∃ x : value α, holds (M ₀↦ x) p
+| M (∀* p)   := ∀ x : denot α, holds (M ₀↦ x) p
+| M (∃* p)   := ∃ x : denot α, holds (M ₀↦ x) p
+
+infix `⊨` : 1000 := holds 
+
+def eqv (α : Type u) (p q : form) : Prop :=
+∀ M : model α, (M ⊨ p ↔ M ⊨ q)
+
+lemma eqv_trans {α : Type u} {p q r : form} :
+  eqv α p q → eqv α q r → eqv α p r :=
+λ h0 h1 M, by rw [h0 M, h1 M]
+
+lemma eqv_refl (α : Type u) (p : form) : eqv α p p := λ M, by refl
+
+namespace form
+
+def size_of : form → nat
+| ⊤*       := 1
+| ⊥*       := 1
+| ⟪_, _⟫   := 1
+| (p ∨* q) := 1 + p.size_of + q.size_of
+| (p ∧* q) := 1 + p.size_of + q.size_of
+| (∀* p)   := 1 + p.size_of
+| (∃* p)   := 1 + p.size_of
+
+instance has_sizeof : has_sizeof form := ⟨size_of⟩ 
+
+/- Increment all variable indices equal to or greater than k by 1. -/
+def incr_idxs_ge : nat → form → form
+| k ⊤*       := ⊤*
+| k ⊥*       := ⊥*
+| k ⟪b, a⟫   := ⟪b, a.incr_idxs_ge k⟫
+| k (p ∨* q) := (incr_idxs_ge k p) ∨* (incr_idxs_ge k q)
+| k (p ∧* q) := (incr_idxs_ge k p) ∧* (incr_idxs_ge k q)
+| k (∀* p)   := ∀* (incr_idxs_ge (k + 1) p)
+| k (∃* p)   := ∃* (incr_idxs_ge (k + 1) p)
+
+def incr_idxs : form → form := incr_idxs_ge 0
+
+def subst : sub → form → form
+| σ ⊤*       := ⊤*
+| σ ⊥*       := ⊥*
+| σ ⟪b, a⟫   := ⟪b, a.subst σ⟫
+| σ (p ∨* q) := (subst σ p) ∨* (subst σ q)
+| σ (p ∧* q) := (subst σ p) ∧* (subst σ q)
+| σ (∀* p)   := ∀* (subst σ.incr_idxs p)
+| σ (∃* p)   := ∃* (subst σ.incr_idxs p)
+
+lemma size_of_subst :
+  ∀ σ : sub, ∀ p : form, (p.subst σ).size_of = p.size_of 
+| σ ⊤*       := rfl
+| σ ⊥*       := rfl
+| σ ⟪b, a⟫   := rfl
+| σ (p ∨* q) := 
+  by simp only [ size_of, subst,
+     size_of_subst σ p, size_of_subst σ q ]
+| σ (p ∧* q) :=
+  by simp only [ size_of, subst,
+     size_of_subst σ p, size_of_subst σ q ]
+| σ (∀* p)   := by simp only [ size_of, subst, size_of_subst _ p ]
+| σ (∃* p)   := by simp only [ size_of, subst, size_of_subst _ p ]
+
+end form
+
+lemma holds_zero_update_incr_idxs {M : model α} {d : denot α} :
+  ∀ p : form, (M ₀↦d) ⊨ p.incr_idxs ↔ M ⊨ p
+| ⊤*       := iff.refl _
+| ⊥*       := iff.refl _
+| ⟪tt, a⟫  := sorry
+| ⟪ff, a⟫  := sorry
+| (q ∨* r) := sorry
+| (q ∧* r) := sorry
+| (∀* q)   := sorry
+| (∃* q)   := sorry
+
+def pull_fa_or_aux : form → form → form
+| p (∀* q) := ∀* (pull_fa_or_aux (p.incr_idxs) q)
+| p      q := p ∨* q
+
+lemma pull_fa_or_aux_eqv  :
+  ∀ p q : form, eqv α (pull_fa_or_aux p q) (p ∨* q)  
+| p ⊤*       := by simp only [pull_fa_or_aux, eqv_refl]
+| p ⊥*       := by simp only [pull_fa_or_aux, eqv_refl]
+| p ⟪b, a⟫   := by simp only [pull_fa_or_aux, eqv_refl]
+| p (q ∨* r) := by simp only [pull_fa_or_aux, eqv_refl]
+| p (q ∧* r) := by simp only [pull_fa_or_aux, eqv_refl]
+| p (∃* q)   := by simp only [pull_fa_or_aux, eqv_refl]
+| p (∀* q)   := 
+  begin
+    intros M, 
+    constructor; intro h0,
+    { cases classical.em (M ⊨ p) with h1 h1,
+      { left, exact h1 },
+      right, intro d, 
+      cases (pull_fa_or_aux_eqv _ q _).elim_left (h0 d) with h2 h2,
+      { cases h1 ((holds_zero_update_incr_idxs p).elim_left h2) },
+      exact h2 },
+    intro d, 
+    rw pull_fa_or_aux_eqv,
+    cases h0,
+    { left, 
+      rw holds_zero_update_incr_idxs, 
+      exact h0 },
+    right, apply h0
+  end
+
+def pull_fa_and_aux : form → form → form
+| p (∀* q) := ∀* (pull_fa_and_aux (p.incr_idxs) q)
+| p      q := p ∧* q
+
+lemma pull_fa_and_aux_eqv [inhabited α] :
+  ∀ p q : form, eqv α (pull_fa_and_aux p q) (p ∧* q)  
+| p ⊤*       := by simp only [pull_fa_and_aux, eqv_refl]
+| p ⊥*       := by simp only [pull_fa_and_aux, eqv_refl]
+| p ⟪b, a⟫   := by simp only [pull_fa_and_aux, eqv_refl]
+| p (q ∨* r) := by simp only [pull_fa_and_aux, eqv_refl]
+| p (q ∧* r) := by simp only [pull_fa_and_aux, eqv_refl]
+| p (∃* q)   := by simp only [pull_fa_and_aux, eqv_refl]
+| p (∀* q)   := 
+  begin
+    intros M, 
+    constructor; intro h0,
+    { refine ⟨_, λ d, _⟩, 
+      { simpa only [holds_zero_update_incr_idxs] using
+        ((pull_fa_and_aux_eqv _ _ _).elim_left
+        (h0 $ denot.default)).left },
+      exact ((pull_fa_and_aux_eqv _ _ _).elim_left (h0 d)).right },
+    intro d,
+    rw pull_fa_and_aux_eqv,
+    refine ⟨(holds_zero_update_incr_idxs _).elim_right h0.left, h0.right _⟩
+  end
+
+def pull_fa_or : form → form → form
+| (∀* p) q := ∀* (pull_fa_or p (q.incr_idxs))
+| p      q := pull_fa_or_aux p  q
+
+lemma pull_fa_or_eqv  :
+  ∀ p q : form, eqv α (pull_fa_or p q) (p ∨* q)  
+| ⊤*       r := by apply pull_fa_or_aux_eqv
+| ⊥*       r := by apply pull_fa_or_aux_eqv
+| ⟪b, a⟫   r := by apply pull_fa_or_aux_eqv
+| (p ∨* q) r := by apply pull_fa_or_aux_eqv
+| (p ∧* q) r := by apply pull_fa_or_aux_eqv
+| (∃* p)   r := by apply pull_fa_or_aux_eqv
+| (∀* p)   r := 
+  begin
+    intros M, 
+    constructor; intro h0,
+    { cases classical.em (M ⊨ r) with h1 h1,
+      { right, exact h1 },
+      left, intro d, 
+      cases (pull_fa_or_eqv _ _ _).elim_left (h0 d) with h2 h2,
+      { exact h2 },
+      cases h1 ((holds_zero_update_incr_idxs r).elim_left h2) },
+    intro d, 
+    rw pull_fa_or_eqv,
+    cases h0,
+    { left, apply h0 },
+    right, 
+    rw holds_zero_update_incr_idxs, 
+    exact h0 
+  end
+
+def pull_fa_and : form → form → form
+| (∀* p) q := ∀* (pull_fa_and p (q.incr_idxs))
+| p      q := pull_fa_and_aux p q
+
+lemma pull_fa_and_eqv [inhabited α] :
+  ∀ p q : form, eqv α (pull_fa_and p q) (p ∧* q)  
+| ⊤*       r := by apply pull_fa_and_aux_eqv
+| ⊥*       r := by apply pull_fa_and_aux_eqv
+| ⟪b, a⟫   r := by apply pull_fa_and_aux_eqv
+| (p ∨* q) r := by apply pull_fa_and_aux_eqv
+| (p ∧* q) r := by apply pull_fa_and_aux_eqv
+| (∃* p)   r := by apply pull_fa_and_aux_eqv
+| (∀* p)   r := 
+  begin
+    intros M, 
+    constructor; intro h0,
+    { refine ⟨λ d, _, _⟩, 
+      { exact ((pull_fa_and_eqv _ _ _).elim_left (h0 d)).left },
+      simpa only [holds_zero_update_incr_idxs] using
+      ((pull_fa_and_eqv _ _ _).elim_left
+      (h0 $ denot.default)).right },
+    intro d,
+    rw pull_fa_and_eqv,
+    refine ⟨h0.left _, (holds_zero_update_incr_idxs _).elim_right h0.right⟩
+  end
+
+def pull_fa_aux : form → form
+| (∀* p) := 
+  have hd : (p.subst [(0, (# 1) & (# 0)), (1, # 0)]).size_of < (∀* p).size_of,
+  { rw form.size_of_subst, 
+    simp only [form.size_of, nat.lt_succ_self, add_comm] }, 
+  ∀* (pull_fa_aux (p.subst [(0, (# 1) & (# 0)), (1, # 0)]))
+| p := ∃* p
+
+def vfo_aux : nat → form → Prop
+| k ⊤*       := true
+| k ⊥*       := true
+| k ⟪b, a⟫   := ¬ head_occ k a 
+| k (p ∨* q) := vfo_aux k p ∧ vfo_aux k q
+| k (p ∧* q) := vfo_aux k p ∧ vfo_aux k q 
+| k (∃* p)   := vfo_aux (k + 1) p
+| k (∀* p)   := vfo_aux (k + 1) p
+
+def vfo : form → Prop
+| ⊤*       := true
+| ⊥*       := true
+| ⟪b, a⟫   := true
+| (p ∨* q) := vfo p ∧ vfo q
+| (p ∧* q) := vfo p ∧ vfo q 
+| (∃* p)   := vfo_aux 0 p ∧ vfo p
+| (∀* p)   := vfo p
+
+
+lemma sub.get_eq_none {σ : sub} {k : nat} : 
+  σ.get k = none → ∀ s : nat × atom, s ∈ σ → k ≠ s.fst := 
+begin
+  intros h0 s h1,
+  unfold sub.get at h0,
+  cases h2 : list.find (eq k ∘ prod.fst) σ,
+  { apply list.find_eq_none.elim_left h2 s h1 },
+  rw h2 at h0, cases h0
+end
+
+
+open list
+
+lemma atom.subst_var_eq {σ : sub} {k : nat} : 
+  (∃ s ∈ σ, k = (s : nat × atom).fst) → 
+  ∃ s ∈ σ, k = (s : nat × atom).fst ∧ (# k).subst σ = (s : nat × atom).snd := 
+begin
+  rintro ⟨s, h0, h1⟩, 
+  cases h2 : find (eq k ∘ prod.fst) σ with t,
+  { cases find_eq_none.elim_left h2 s h0 h1 },
+  refine ⟨t, find_mem h2, ⟨_, _⟩⟩, 
+  { apply find_some h2 },
+  simp only [atom.subst, sub.get, h2, option.map_some]
+end
+
+lemma atom.subst_var_eq_self {σ : sub} {k : nat} : 
+  ¬ (∃ s ∈ σ, k = (s : nat × atom).fst) → (# k).subst σ = # k := 
+begin
+  intro h0,
+  unfold atom.subst, unfold sub.get,
+  cases h2 : find (eq k ∘ prod.fst) σ with t, refl, 
+  cases (h0 ⟨t, find_mem h2, _⟩  : false),
+  apply find_some h2
+end
+
+lemma nat.ne_succ (n : nat) : n ≠ n.succ := sorry
+
+
+
+
+lemma not_head_occ_subst (k m : nat) :
+  head_occ k (atom.subst [(k, (# (k + 1) & (# k))), (k + 1, # k)] (# m))
+  → head_occ (k + 1) (# m) :=
+begin
+
+end
+
+#exit
+lemma not_head_occ_subst (k : nat) :
+   ∀ a : atom, ¬head_occ (k + 1) a → 
+  ¬ head_occ k (atom.subst [(k, (# (k + 1) & (# k))), (k + 1, # k)] a)
+| (# m) h0 :=
+  begin
+    by_cases h1 : (∃ s ∈ [(k, (# (k + 1) & (# k))), 
+      (k + 1, # k)], m = (s : nat × atom).fst),
+    { rcases atom.subst_var_eq h1 with ⟨s, h2, h3, h4⟩, 
+      rw h4, 
+      rw mem_cons_iff at h2, cases h2,
+      { rw h2, apply nat.ne_succ },
+      rw mem_singleton at h2,
+      rw [h3, h2] at h0,
+      cases (h0 rfl : false) },
+    rw atom.subst_var_eq_self h1,
+    intro hc,
+    apply h1 ⟨_, or.inl rfl, hc.symm⟩
+  end
+| (a & (# m)) h0 :=
+  begin
+    intro h1, apply not_head_occ_subst a h0 _,
+    simp only [atom.subst] at h1, 
+    
+  end
+
+
+#exit
+lemma vfo_aux_subst : 
+  ∀ k : nat, ∀ p : form, vfo_aux (k + 1) p → 
+   vfo_aux k (form.subst [(0, (# 1) & (# 0)), (1, # 0)] p) 
+| k ⊤*       h0 := trivial
+| k ⊥*       h0 := trivial
+| k ⟪b, a⟫   h0 := 
+  begin
+   simp [vfo_aux, form.subst] at *,
+  end
+| k (p ∨* q) h0 := sorry
+| k (p ∧* q) h0 := sorry
+| k (∃* p)   h0 := sorry
+| k (∀* p)   h0 := sorry
+
+#exit
+lemma vfo_subst {p : form} (σ : sub) :
+  vfo p → vfo (p.subst σ) := sorry
+
+lemma pull_fa_aux_eqv :
+  ∀ p : form, vfo (∃* p) → eqv α (pull_fa_aux p) (∃* p)
+| ⊤*       fh := by simp only [pull_fa_aux, eqv_refl]
+| ⊥*       fh := by simp only [pull_fa_aux, eqv_refl]
+| ⟪b, a⟫   fh := by simp only [pull_fa_aux, eqv_refl]
+| (p ∨* q) fh := by simp only [pull_fa_aux, eqv_refl]
+| (p ∧* q) fh := by simp only [pull_fa_aux, eqv_refl]
+| (∃* p)   fh := by simp only [pull_fa_aux, eqv_refl]
+| (∀* p)   fh := 
+  have hd : (p.subst [(0, # 1&# 0), (1, # 0)]).size_of < (∀* p).size_of,
+  { admit },
+  begin
+    simp [pull_fa_aux],
+    have h0 := pull_fa_aux_eqv (p.subst [(0, # 1&# 0), (1, # 0)]),
+    apply @eqv_trans α _ (∀* $ ∃* (p.subst [(0, # 1&# 0), (1, # 0)])),
+    { intro M, constructor; intros h1 d,
+      { apply (h0 ⟨_, _⟩ _).elim_left (h1 _),
+      cases fh,
+      
+         },
+      apply (h0 _ _).elim_right (h1 _) },
+
+    intro M, constructor; intro h1,
+    { apply classical.by_contradiction, intro hc,
+      have h2 : ∀ d : denot α, ∃ e : denot α, ¬ ((M ₀↦ d) ₀↦ e) ⊨ p,
+      { admit },
+
+
+
+    
+     }
+
+  end
+
+#check @eqv_trans
+
+#exit
+def pull_fa : form → form
+| (p ∨* q) := pull_fa_fork (∨*) (pull_fa p) (pull_fa q) 
+| (p ∧* q) := pull_fa_fork (∧*) (pull_fa p) (pull_fa q) 
+| (∀* p)   := ∀* (pull_fa p)
+| (∃* p)   := pull_fa_aux (pull_fa p)
+| p        := p
+
+#exit
+def pnf_right (c : form → form → form) : form → form → form
+| p (∀* q) := ∀* (pnf_right (p.incr_idxs 0) q)
+| p (∃* q) := ∃* (pnf_right (p.incr_idxs 0) q)
+| p      q := c p q
+
+def pnf_left (c : form → form → form) : form → form → form
+| (∀* p) q := ∀* (pnf_left p (q.incr_idxs 0))
+| (∃* p) q := ∃* (pnf_left p (q.incr_idxs 0))
+| p      q := pnf_right c p q
+
+def pnf : form → form
+| ⊤*       := ⊤*
+| ⊥*       := ⊥*
+| ⟪l⟫      := ⟪l⟫
+| (p ∨* q) := pnf_left (∨*) (pnf p) (pnf q)
+| (p ∧* q) := pnf_left (∧*) (pnf p) (pnf q)
+| (∀* p)   := ∀* (pnf p)
+| (∃* p)   := ∃* (pnf p)
